src/3d/Z3TestGen.fst
@@ -923,7 +923,7 @@ let rec typ_depth (t: I.typ) : GTot nat
   | I.T_with_comment _ t' _
   | I.T_at_most _ _ t'
   | I.T_exact _ _ t'
-  | I.T_nlist _ _ t'
+  | I.T_nlist _ _ _ t'
     -> 1 + typ_depth t'
   | I.T_with_dep_action _ _ _
   | I.T_refine _ _ _
@@ -955,7 +955,7 @@ let rec parse_typ (t : I.typ) : Tot (parser not_reading)
   | I.T_at_most _ size body -> parse_at_most (fun _ -> mk_expr size) (parse_typ body)
   | I.T_exact _ size body -> parse_exact (fun _ -> mk_expr size) (parse_typ body)
   | I.T_string _ elt terminator -> parse_string (parse_readable_dtyp elt) (fun _ -> mk_expr terminator)
-  | I.T_nlist _ size body ->
+  | I.T_nlist _ _ size body ->
     if match body with
     | I.T_denoted _ (I.DT_IType i) -> Some? (itype_byte_size i)
     | _ -> false
